\section{}
Compute the matrix exponential

\[
    e^{At}, \; A = 
    \begin{bmatrix}
        2 & -1 \\ 
        -1 & 2
    \end{bmatrix}
\]

\subsection{}
\textit{By hand calculations (start by solving for the eigenvalues and eigenvectors of A)}

First we solve for the eigenvalues of $A$:
\[
    \begin{aligned}
        \det(A - \lambda I) &= 0 \\
        \det
        \begin{bmatrix}
            2 - \lambda & -1 \\
            -1 & 2 - \lambda
        \end{bmatrix} &= 0 \\
        (2 - \lambda)^2 - 1 &= 0 \\
        \lambda & = 2 \pm 1 \\
        \lambda & = 1, 3
    \end{aligned}
\]

Next, we solve for the eigenvectors of $A$. First for $\lambda = 1$:
\[
    \begin{aligned}
        (A - \lambda I) v &= 0 \\
        \begin{bmatrix}
            1 & -1 \\
            -1 & 1
        \end{bmatrix} v &= 0 \\
    \end{aligned}
\]

Since the system is underdetermined, we can let $v_1 = \alpha$, then

\[
    \begin{aligned}
        v_2 &= v_1 \\
        v &= \alpha
        \begin{bmatrix}
            1 \\
            1
        \end{bmatrix}
    \end{aligned}
\]

Next, for $\lambda = 3$:
\[
    \begin{aligned}
        (A - \lambda I) v &= 0 \\
        \begin{bmatrix}
            -1 & -1 \\
            -1 & -1
        \end{bmatrix} v &= 0 \\
    \end{aligned}
\]
Again, since the system is underdetermined, we can let $v_1 = \beta$, then
\[
    \begin{aligned}
        v_2 &= -v_1 \\
        v &= \beta
        \begin{bmatrix}
            1 \\
            -1
        \end{bmatrix}
    \end{aligned}
\]

Therefore, the D and V matrices are
\[
    D = 
    \begin{bmatrix}
        1 & 0 \\
        0 & 3
    \end{bmatrix}
    , \;
    V = 
    \begin{bmatrix}
        1 & 1 \\
        1 & -1
    \end{bmatrix}
\]

Next, determine $V^{-1}$:
\[
    \begin{aligned}
        V^{-1} &= \frac{1}{\det(V)} \text{adj}(V) \\
        &= \frac{1}{-2} 
        \begin{bmatrix}
            -1 & -1 \\
            -1 & 1
        \end{bmatrix} \\
        &= 
        \begin{bmatrix}
            \frac{1}{2} & \frac{1}{2} \\
            \frac{1}{2} & -\frac{1}{2}
        \end{bmatrix}
    \end{aligned}
\]

Next, evaluating $e^{Dt}$ by the special case of diagonal matrices:
\[
    \begin{aligned}
        e^{Dt} &= 
        \begin{bmatrix}
            e^{D_{11}t} & 0 \\
            0 & e^{D_{22}t}
        \end{bmatrix} \\
        &= 
        \begin{bmatrix}
            e^t & 0 \\
            0 & e^{3t}
        \end{bmatrix}
    \end{aligned}
\]

Finally, we can solve for $e^{At}$:
\[
    \begin{aligned}
        e^{At} &= V e^{Dt} V^{-1} \\
        &= 
        \begin{bmatrix}
            1 & 1 \\
            1 & -1
        \end{bmatrix}
        \begin{bmatrix}
            e^t & 0 \\
            0 & e^{3t}
        \end{bmatrix}
        \begin{bmatrix}
            \frac{1}{2} & \frac{1}{2} \\
            \frac{1}{2} & -\frac{1}{2}
        \end{bmatrix} \\
        &= 
        \begin{bmatrix}
            e^t & e^{3t} \\
            e^t & -e^{3t}
        \end{bmatrix} 
        \begin{bmatrix}
            \frac{1}{2} & \frac{1}{2} \\
            \frac{1}{2} & -\frac{1}{2}
        \end{bmatrix} \\
        &=
        \begin{bmatrix}
            \frac{e^t + e^{3t}}{2} & \frac{e^t - e^{3t}}{2} \\
            \frac{e^t - e^{3t}}{2} & \frac{e^t + e^{3t}}{2}
        \end{bmatrix} \\
        &= 
        \frac{1}{2}
        \begin{bmatrix}
            e^t + e^{3t} & e^t - e^{3t} \\
            e^t - e^{3t} & e^t + e^{3t}
        \end{bmatrix}
    \end{aligned}
\]

So,
\begin{empheq}[box=\fbox]{align*}
    e^{At} &= 
    \frac{1}{2}
    \begin{bmatrix}
        e^t + e^{3t} & e^t - e^{3t} \\
        e^t - e^{3t} & e^t + e^{3t}
    \end{bmatrix}
\end{empheq}

\subsection{}
\textit{Using MATLAB}

Using the Matlab code:
\lstinputlisting[language=Matlab]{Questions/Code/a2q3.m}

The output is 

\texttt{
    >>> ans = \\
    \hspace*{2em} [exp(3*t)/2 + exp(t)/2, exp(t)/2 - exp(3*t)/2] \\
    \hspace*{2em} [exp(t)/2 - exp(3*t)/2, exp(3*t)/2 + exp(t)/2]
}

Which is the same as the answer from part (a).